Avance dans la decidabilite du typage des patches.
git-svn-id: http://gasp.dev.regis-gianas.com/svn/trunk@33 403e655e-980a-47bd-8c60-1ee5348bb6b7

coq/stlc.v
@@ -1,3 +1,5 @@
+(* Simply Type Lambda-Calculus, formalized *)
+
 Inductive type : Type :=
 | base
 | arr (A B : type).
@@ -8,19 +10,29 @@ Inductive term : Type :=
 | lam (x : nat) (A : type) (t : term).
 
 Inductive env : Type :=
-| nil
-| cons (x : nat) (A : type) (tl : env).
+| enil
+| econs (x : nat) (A : type) (tl : env).
 
 Inductive lookup (x : nat) (A : type) : env -> Type :=
-| look_it {tl} : lookup x A (cons x A tl)
-| look_next {y B tl} : lookup x A tl -> lookup x A (cons y B tl).
+| look_it {tl} : lookup x A (econs x A tl)
+| look_next {y B tl} : lookup x A tl -> lookup x A (econs y B tl).
 
 Inductive of : env -> term -> type -> Type :=
 | Var {Γ} x {A} : lookup x A Γ -> of Γ (var x) A
 | App {Γ t u} A {B} : of Γ t (arr A B) -> of Γ u A -> of Γ (app t u) B
-| Lam {Γ x t A B} : of (cons x A Γ) t B -> of Γ (lam x A t) (arr A B).
+| Lam {Γ x t A B} : of (econs x A Γ) t B -> of Γ (lam x A t) (arr A B).
 
 Require Import data_meta.
+Require Import Peano_dec.
+
+Module V <: VAR.
+  Definition var := nat.
+  Definition var_eq_dec := eq_nat_dec.
+End V.
+
+Import V.
+
+(* We now define atoms and transformers *)
 
 Inductive atom := 
 | Atype
@@ -29,13 +41,51 @@ Inductive atom :=
 | Alookup (x A E : var)
 | Aof (E t A : var).
 
+Definition atom_eq_dec : eq_dec atom.
+red; intros; destruct x; destruct y;
+(left; reflexivity) || (right; discriminate) || idtac.
+case (var_eq_dec x x0); case(var_eq_dec A A0); case(var_eq_dec E E0);
+intros; subst; auto; right; intro H; injection H; contradiction.
+case (var_eq_dec t t0); case(var_eq_dec A A0); case(var_eq_dec E E0);
+intros; subst; auto; right; intro H; injection H; contradiction.
+Qed.
+
 Inductive transformer :=
 | Tbase | Tarr | Tvar | Tapp | Tlam | Tnil | Tcons 
 | Tlook_it | Tlook_next | TVar | TApp | TLam.
 
-Module L : LANG.
+Lemma transformer_eq_dec : eq_dec transformer.
+red; intros. destruct x; destruct y;
+(left; reflexivity) || (right; discriminate).
+Qed.
+
+
+Module L <: LANG.
   Definition atom := atom.
+  Definition atom_eq_dec := atom_eq_dec.
   Definition transformer := transformer.
+  Definition transformer_eq_dec := transformer_eq_dec.
 End L.
 
-Module PL := Patch L.
+(* We can apply the functor *)
+
+Module PL := Patch L V.
+Import PL.
+
+(* Some example transformer arities. Their creation should be
+automatizable in Ltac. *)
+
+Definition Sbase := pair Tbase 
+  {| ar_args := List.nil; 
+     ar_concls := Jdecl {| d_var := 1; d_params := nil; d_atom := Atype  |} :: nil
+  |}.
+
+Definition Sarr := pair Tarr
+  {| ar_args := Jdecl {| d_var := 1; d_params := nil; d_atom := Atype |} :: nil;
+     ar_concls := Jdecl {| d_var := 2; d_params := nil; d_atom := Atype |} :: nil
+  |}.
+
+Definition Svar := pair Tvar
+  {| ar_args := Jdecl {| d_var := 1; d_params := nil; d_atom := Atype |} :: nil;
+     ar_concls := Jdecl {| d_var := 2; d_params := nil; d_atom := Atype |} :: nil
+  |}.
